theories/rules/rules_Store.v
@@ -73,8 +73,9 @@ Section cap_lang_rules.
   | Store_fail_invalid_locality p g b e a storev:
       regs !! r1 = Some(inr ((p, g), b, e, a)) ->
       word_of_argument regs r2 = Some storev ->
-      isLocalWord storev = true →
-      pwl p = false →
+      canStore p a storev = false ->
+      (* isLocalWord storev = true → *)
+      (* pwl p = false → *)
       Store_failure regs r1 r2 mem
   | Store_fail_invalid_PC:
       incrementPC (regs) = None ->
@@ -251,27 +252,40 @@ Section cap_lang_rules.
        rewrite -Hr0 in Hregs0; rewrite Hregs0 in HSV. exact HSV.
      }
 
-     destruct (decide (isLocalWord storev = true ∧ pwl p = false)).
-     {  (* Failure: trying to write a local value to a non-WL cap *)
-            destruct a0 as [HLW Hpwl].
-       assert (c = Failed ∧ σ2 = (r, m)) as (-> & ->).
-      { destruct storev.
-       - cbv in HLW; by exfalso.
-       - destruct (word_of_argument_inr _ _ _ HSVr) as (r0 & -> & Hr0s).
-         destruct (isLocalWord_cap_isLocal _ HLW) as (p' & g' & b' & e' & a' & -> & HIL).
-         option_locate_mr m r. rewrite /canStore Hrr0 HIL in Hstep.
-         destruct p; try by exfalso. all: by inversion Hstep.
-      }
-      iFailWP "Hφ" Store_fail_invalid_locality.
+     case_eq (canStore p a storev); intro HcanStore.
+     2:{ destruct r2.
+         - simpl in HSV; inv HSV. simpl in HcanStore; congruence.
+         - assert (c = Failed ∧ σ2 = (r, m)) as (-> & ->).
+           { simpl in HSV; inv HSV. rewrite /= in HSVr.
+             rewrite /= /RegLocate in Hstep.
+             destruct (r !! r0); try congruence. inv HSVr.
+             rewrite HcanStore in Hstep. inv Hstep; auto. }
+           iFailWP "Hφ" Store_fail_invalid_locality.
      }
 
+
+     (* destruct (decide (isLocalWord storev = true ∧ pwl p = false)). *)
+     (* {  (* Failure: trying to write a local value to a non-WL cap *) *)
+     (*        destruct a0 as [HLW Hpwl]. *)
+     (*   assert (c = Failed ∧ σ2 = (r, m)) as (-> & ->). *)
+     (*  { destruct storev. *)
+     (*   - cbv in HLW; by exfalso. *)
+     (*   - destruct (word_of_argument_inr _ _ _ HSVr) as (r0 & -> & Hr0s). *)
+     (*     destruct (isLocalWord_cap_isLocal _ HLW) as (p' & g' & b' & e' & a' & -> & HIL). *)
+     (*     option_locate_mr m r. rewrite /canStore  Hrr0 /= Hpwl in Hstep. *)
+     (*     destruct g'; simpl in HIL; try congruence; inversion Hstep; auto. } *)
+     (*  iFailWP "Hφ" Store_fail_invalid_locality. *)
+     (* } *)
+
      assert (isLocalWord storev = false ∨ pwl p = true) as HLocal.
-     {
-     apply (not_and_r) in n0.
-     destruct n0 as [Hlw | Hpwl].
-     destruct (isLocalWord storev); first by exfalso. by left.
-     destruct (pwl p); last by exfalso. by right.
-     } clear n0.
+     { rewrite /canStore in HcanStore. destruct storev; simpl; auto.
+       destruct_cap c0. destruct c4; auto.
+       eapply andb_true_iff in HcanStore. destruct HcanStore; auto. }
+     (* apply (not_and_r) in n0. *)
+     (* destruct n0 as [Hlw | Hpwl]. *)
+     (* destruct (isLocalWord storev); first by exfalso. by left. *)
+     (* destruct (pwl p); last by exfalso. by right. *)
+     (* } clear n0. *)
 
      (* Prove that a is in the memory map now, otherwise we cannot continue *)
      pose proof (allow_store_implies_storev r1 r2 mem regs p g b e a storev) as (p' & oldv & Hmema & HPFp); auto.
@@ -295,12 +309,8 @@ Section cap_lang_rules.
            epose proof (regs_lookup_inr_eq r r0 _ _ _ _ _ Hr0) as Hr0'.
            simpl in HSVr; rewrite Hr0' in HSVr; inversion HSVr.
            subst storev; clear HSVr.
-           destruct HLocal as [HiLW | Hpwl].
-           + cbv in HiLW. destruct c4; last by exfalso. simpl in Hstep. done.
-           + destruct c4; simpl in Hstep.
-             ++ done.
-             ++ apply pwl_implies_RWL_RWLX in Hpwl.
-                destruct Hpwl as [-> | ->]; done.
+           rewrite HcanStore /= in Hstep.
+           auto.
        }
       iMod ((gen_mem_update_inSepM _ _ a) with "Hm Hmem") as "[Hm Hmem]"; eauto.
 
@@ -370,96 +380,96 @@ Section cap_lang_rules.
      }
    Qed.
 
-   Lemma wp_store_success_reg_PC E src wsrc pc_p pc_p' pc_g pc_b pc_e pc_a pc_a' w :
-     decodeInstrW w = Store PC (inr src) →
-     PermFlows pc_p pc_p' →
-     isCorrectPC (inr ((pc_p,pc_g),pc_b,pc_e,pc_a)) →
-     (pc_a + 1)%a = Some pc_a' →
-     writeAllowed pc_p = true →
-     (isLocalWord wsrc = false ∨ (pc_p = RWL ∨ pc_p = RWLX)) ->
+   (* Lemma wp_store_success_reg_PC E src wsrc pc_p pc_p' pc_g pc_b pc_e pc_a pc_a' w : *)
+   (*   decodeInstrW w = Store PC (inr src) → *)
+   (*   PermFlows pc_p pc_p' → *)
+   (*   isCorrectPC (inr ((pc_p,pc_g),pc_b,pc_e,pc_a)) → *)
+   (*   (pc_a + 1)%a = Some pc_a' → *)
+   (*   writeAllowed pc_p = true → *)
+   (*   (isLocalWord wsrc = false ∨ (pc_p = RWL ∨ pc_p = RWLX)) -> *)
 
-     {{{ ▷ PC ↦ᵣ inr ((pc_p,pc_g),pc_b,pc_e,pc_a)
-           ∗ ▷ pc_a ↦ₐ[pc_p'] w
-           ∗ ▷ src ↦ᵣ wsrc }}}
-       Instr Executable @ E
-       {{{ RET NextIV;
-           PC ↦ᵣ inr ((pc_p,pc_g),pc_b,pc_e,pc_a')
-              ∗ pc_a ↦ₐ[pc_p'] wsrc
-              ∗ src ↦ᵣ wsrc }}}.
-   Proof.
-     iIntros (Hinstr Hfl Hvpc Hpca' Hwa Hloc φ)
-            "(>HPC & >Hi & >Hsrc) Hφ".
-     iDestruct (map_of_regs_2 with "HPC Hsrc") as "[Hmap %]".
-     iDestruct (memMap_resource_1 with "Hi") as "Hmem".
+   (*   {{{ ▷ PC ↦ᵣ inr ((pc_p,pc_g),pc_b,pc_e,pc_a) *)
+   (*         ∗ ▷ pc_a ↦ₐ[pc_p'] w *)
+   (*         ∗ ▷ src ↦ᵣ wsrc }}} *)
+   (*     Instr Executable @ E *)
+   (*     {{{ RET NextIV; *)
+   (*         PC ↦ᵣ inr ((pc_p,pc_g),pc_b,pc_e,pc_a') *)
+   (*            ∗ pc_a ↦ₐ[pc_p'] wsrc *)
+   (*            ∗ src ↦ᵣ wsrc }}}. *)
+   (* Proof. *)
+   (*   iIntros (Hinstr Hfl Hvpc Hpca' Hwa Hloc φ) *)
+   (*          "(>HPC & >Hi & >Hsrc) Hφ". *)
+   (*   iDestruct (map_of_regs_2 with "HPC Hsrc") as "[Hmap %]". *)
+   (*   iDestruct (memMap_resource_1 with "Hi") as "Hmem". *)
 
-    iApply (wp_store with "[$Hmap $Hmem]"); eauto; simplify_map_eq; eauto.
-    { by rewrite !dom_insert; set_solver+. }
-    { eapply mem_eq_implies_allow_store_map; eauto.
-      all: by simplify_map_eq. }
-    iNext. iIntros (regs' mem' retv) "(#Hspec & Hmem & Hmap)".
-    iDestruct "Hspec" as %Hspec.
+   (*  iApply (wp_store with "[$Hmap $Hmem]"); eauto; simplify_map_eq; eauto. *)
+   (*  { by rewrite !dom_insert; set_solver+. } *)
+   (*  { eapply mem_eq_implies_allow_store_map; eauto. *)
+   (*    all: by simplify_map_eq. } *)
+   (*  iNext. iIntros (regs' mem' retv) "(#Hspec & Hmem & Hmap)". *)
+   (*  iDestruct "Hspec" as %Hspec. *)
 
-    destruct Hspec as [ | * Hfail ].
-     { (* Success *)
-       iApply "Hφ".
-       destruct H4 as [Hrr2 _]. simplify_map_eq.
-       rewrite memMap_resource_1.
-       incrementPC_inv.
-       simplify_map_eq.
-       do 2 rewrite insert_insert.
-       iDestruct (regs_of_map_2 with "[$Hmap]") as "[HPC Hsrc]"; eauto. iFrame. }
-     { (* Failure (contradiction) *)
-       destruct Hfail; try incrementPC_inv; simplify_map_eq; eauto.
-       - apply isCorrectPC_ra_wb in Hvpc. apply andb_prop_elim in Hvpc as [_ Hwb].
-         destruct o; last apply Is_true_false in H3; congruence.
-       - destruct Hloc; first congruence. naive_solver.
-       - congruence.
-     }
-    Qed.
+   (*  destruct Hspec as [ | * Hfail ]. *)
+   (*   { (* Success *) *)
+   (*     iApply "Hφ". *)
+   (*     destruct H4 as [Hrr2 _]. simplify_map_eq. *)
+   (*     rewrite memMap_resource_1. *)
+   (*     incrementPC_inv. *)
+   (*     simplify_map_eq. *)
+   (*     do 2 rewrite insert_insert. *)
+   (*     iDestruct (regs_of_map_2 with "[$Hmap]") as "[HPC Hsrc]"; eauto. iFrame. } *)
+   (*   { (* Failure (contradiction) *) *)
+   (*     destruct Hfail; try incrementPC_inv; simplify_map_eq; eauto. *)
+   (*     - apply isCorrectPC_ra_wb in Hvpc. apply andb_prop_elim in Hvpc as [_ Hwb]. *)
+   (*       destruct o; last apply Is_true_false in H3; congruence. *)
+   (*     - destruct Hloc; first congruence. naive_solver. *)
+   (*     - congruence. *)
+   (*   } *)
+   (*  Qed. *)
 
-   Lemma wp_store_success_reg_PC_same E pc_p pc_g pc_b pc_e pc_a pc_a' w w' pc_p' :
-     decodeInstrW w = Store PC (inr PC) →
-     PermFlows pc_p pc_p' →
-     isCorrectPC (inr ((pc_p,pc_g),pc_b,pc_e,pc_a)) →
-     (pc_a + 1)%a = Some pc_a' →
-     writeAllowed pc_p = true →
-     (isLocal pc_g = false ∨ (pc_p = RWLX ∨ pc_p = RWL)) →
+   (* Lemma wp_store_success_reg_PC_same E pc_p pc_g pc_b pc_e pc_a pc_a' w w' pc_p' : *)
+   (*   decodeInstrW w = Store PC (inr PC) → *)
+   (*   PermFlows pc_p pc_p' → *)
+   (*   isCorrectPC (inr ((pc_p,pc_g),pc_b,pc_e,pc_a)) → *)
+   (*   (pc_a + 1)%a = Some pc_a' → *)
+   (*   writeAllowed pc_p = true → *)
+   (*   (isLocal pc_g = false ∨ (pc_p = RWLX ∨ pc_p = RWL)) → *)
 
-     {{{ ▷ PC ↦ᵣ inr ((pc_p,pc_g),pc_b,pc_e,pc_a)
-           ∗ ▷ pc_a ↦ₐ[pc_p'] w }}}
-       Instr Executable @ E
-       {{{ RET NextIV;
-           PC ↦ᵣ inr ((pc_p,pc_g),pc_b,pc_e,pc_a')
-              ∗ pc_a ↦ₐ[pc_p'] inr ((pc_p,pc_g),pc_b,pc_e,pc_a) }}}.
-   Proof.
-     iIntros (Hinstr Hfl Hvpc Hpca' Hwa Hloc φ)
-            "(>HPC & >Hi) Hφ".
-     iDestruct (map_of_regs_1 with "HPC") as "Hmap".
-     iDestruct (memMap_resource_1 with "Hi") as "Hmem".
+   (*   {{{ ▷ PC ↦ᵣ inr ((pc_p,pc_g),pc_b,pc_e,pc_a) *)
+   (*         ∗ ▷ pc_a ↦ₐ[pc_p'] w }}} *)
+   (*     Instr Executable @ E *)
+   (*     {{{ RET NextIV; *)
+   (*         PC ↦ᵣ inr ((pc_p,pc_g),pc_b,pc_e,pc_a') *)
+   (*            ∗ pc_a ↦ₐ[pc_p'] inr ((pc_p,pc_g),pc_b,pc_e,pc_a) }}}. *)
+   (* Proof. *)
+   (*   iIntros (Hinstr Hfl Hvpc Hpca' Hwa Hloc φ) *)
+   (*          "(>HPC & >Hi) Hφ". *)
+   (*   iDestruct (map_of_regs_1 with "HPC") as "Hmap". *)
+   (*   iDestruct (memMap_resource_1 with "Hi") as "Hmem". *)
 
-    iApply (wp_store with "[$Hmap $Hmem]"); eauto; simplify_map_eq; eauto.
-    { by rewrite !dom_insert; set_solver+. }
-    { eapply mem_eq_implies_allow_store_map; eauto.
-      all: by simplify_map_eq. }
-    iNext. iIntros (regs' mem' retv) "(#Hspec & Hmem & Hmap)".
-    iDestruct "Hspec" as %Hspec.
+   (*  iApply (wp_store with "[$Hmap $Hmem]"); eauto; simplify_map_eq; eauto. *)
+   (*  { by rewrite !dom_insert; set_solver+. } *)
+   (*  { eapply mem_eq_implies_allow_store_map; eauto. *)
+   (*    all: by simplify_map_eq. } *)
+   (*  iNext. iIntros (regs' mem' retv) "(#Hspec & Hmem & Hmap)". *)
+   (*  iDestruct "Hspec" as %Hspec. *)
 
-    destruct Hspec as [ | * Hfail ].
-     { (* Success *)
-       iApply "Hφ".
-       destruct H3 as [Hrr2 _]. simplify_map_eq.
-       rewrite memMap_resource_1.
-       incrementPC_inv.
-       simplify_map_eq.
-       do 2 rewrite insert_insert.
-       iDestruct (regs_of_map_1 with "[$Hmap]") as "HPC"; eauto. iFrame. }
-     { (* Failure (contradiction) *)
-       destruct Hfail; try incrementPC_inv; simplify_map_eq; eauto. destruct o . all: try congruence.
-       - apply isCorrectPC_ra_wb in Hvpc. apply andb_prop_elim in Hvpc as [_ Hwb].
-         apply Is_true_false in H2; congruence.
-       - destruct Hloc; first congruence. naive_solver.
-     }
-    Qed.
+   (*  destruct Hspec as [ | * Hfail ]. *)
+   (*   { (* Success *) *)
+   (*     iApply "Hφ". *)
+   (*     destruct H3 as [Hrr2 _]. simplify_map_eq. *)
+   (*     rewrite memMap_resource_1. *)
+   (*     incrementPC_inv. *)
+   (*     simplify_map_eq. *)
+   (*     do 2 rewrite insert_insert. *)
+   (*     iDestruct (regs_of_map_1 with "[$Hmap]") as "HPC"; eauto. iFrame. } *)
+   (*   { (* Failure (contradiction) *) *)
+   (*     destruct Hfail; try incrementPC_inv; simplify_map_eq; eauto. destruct o . all: try congruence. *)
+   (*     - apply isCorrectPC_ra_wb in Hvpc. apply andb_prop_elim in Hvpc as [_ Hwb]. *)
+   (*       apply Is_true_false in H2; congruence. *)
+   (*     - destruct Hloc; first congruence. naive_solver. *)
+   (*   } *)
+   (*  Qed. *)
 
    Lemma wp_store_success_same E pc_p pc_g pc_b pc_e pc_a pc_a' w dst z w'
          p g b e pc_p' :
@@ -504,277 +514,277 @@ Section cap_lang_rules.
        destruct Hfail; try incrementPC_inv; simplify_map_eq; eauto.
        destruct o. all: congruence.
      }
-     Qed.
+    Qed.
 
-   Lemma wp_store_success_reg' E pc_p pc_g pc_b pc_e pc_a pc_a' w dst w'
-         p g b e a pc_p' p' :
-      decodeInstrW w = Store dst (inr PC) →
-      PermFlows pc_p pc_p' →
-     isCorrectPC (inr ((pc_p,pc_g),pc_b,pc_e,pc_a)) →
-     (pc_a + 1)%a = Some pc_a' →
-     writeAllowed p = true ∧ withinBounds ((p, g), b, e, a) = true →
-     (isLocal pc_g = false ∨ (p = RWLX ∨ p = RWL)) →
+   (* Lemma wp_store_success_reg' E pc_p pc_g pc_b pc_e pc_a pc_a' w dst w' *)
+   (*       p g b e a pc_p' p' : *)
+   (*    decodeInstrW w = Store dst (inr PC) → *)
+   (*    PermFlows pc_p pc_p' → *)
+   (*   isCorrectPC (inr ((pc_p,pc_g),pc_b,pc_e,pc_a)) → *)
+   (*   (pc_a + 1)%a = Some pc_a' → *)
+   (*   writeAllowed p = true ∧ withinBounds ((p, g), b, e, a) = true → *)
+   (*   (isLocal pc_g = false ∨ (p = RWLX ∨ p = RWL)) → *)
 
-     {{{ ▷ PC ↦ᵣ inr ((pc_p,pc_g),pc_b,pc_e,pc_a)
-           ∗ ▷ pc_a ↦ₐ[pc_p'] w
-           ∗ ▷ dst ↦ᵣ inr ((p,g),b,e,a)
-           ∗ if (a =? pc_a)%a
-             then ⌜PermFlows p pc_p'⌝
-             else ⌜PermFlows p p'⌝ ∗ ▷ a ↦ₐ[p'] w' }}}
-       Instr Executable @ E
-       {{{ RET NextIV;
-           PC ↦ᵣ inr ((pc_p,pc_g),pc_b,pc_e,pc_a')
-              ∗ pc_a ↦ₐ[pc_p'] (if (a =? pc_a)%a
-                               then (inr ((pc_p,pc_g),pc_b,pc_e,pc_a))
-                               else w)
-              ∗ dst ↦ᵣ inr ((p,g),b,e,a)
-              ∗ if (a =? pc_a)%a
-                then emp
-                else a ↦ₐ[p'] (inr ((pc_p,pc_g),pc_b,pc_e,pc_a)) }}}.
-   Proof.
-     iIntros (Hinstr Hfl Hvpc Hpca' [Hwa Hwb] Hloc φ)
-            "(>HPC & >Hi & >Hdst & Ha) Hφ".
-     iDestruct (map_of_regs_2 with "HPC Hdst") as "[Hmap %]".
-     iDestruct (extract_sep_if_split with "Ha") as "[Hflt Hr1a]".
-     iAssert (⌜if (a =? pc_a)%a then PermFlows p pc_p' else PermFlows p p'⌝)%I with "[Hflt]" as %Hfl'.
-     { iRevert "Hflt". destruct (a =? pc_a)%a; auto. }
-     iDestruct (memMap_resource_2gen_clater with "Hi Hr1a") as (mem) "[>Hmem %]".
+   (*   {{{ ▷ PC ↦ᵣ inr ((pc_p,pc_g),pc_b,pc_e,pc_a) *)
+   (*         ∗ ▷ pc_a ↦ₐ[pc_p'] w *)
+   (*         ∗ ▷ dst ↦ᵣ inr ((p,g),b,e,a) *)
+   (*         ∗ if (a =? pc_a)%a *)
+   (*           then ⌜PermFlows p pc_p'⌝ *)
+   (*           else ⌜PermFlows p p'⌝ ∗ ▷ a ↦ₐ[p'] w' }}} *)
+   (*     Instr Executable @ E *)
+   (*     {{{ RET NextIV; *)
+   (*         PC ↦ᵣ inr ((pc_p,pc_g),pc_b,pc_e,pc_a') *)
+   (*            ∗ pc_a ↦ₐ[pc_p'] (if (a =? pc_a)%a *)
+   (*                             then (inr ((pc_p,pc_g),pc_b,pc_e,pc_a)) *)
+   (*                             else w) *)
+   (*            ∗ dst ↦ᵣ inr ((p,g),b,e,a) *)
+   (*            ∗ if (a =? pc_a)%a *)
+   (*              then emp *)
+   (*              else a ↦ₐ[p'] (inr ((pc_p,pc_g),pc_b,pc_e,pc_a)) }}}. *)
+   (* Proof. *)
+   (*   iIntros (Hinstr Hfl Hvpc Hpca' [Hwa Hwb] Hloc φ) *)
+   (*          "(>HPC & >Hi & >Hdst & Ha) Hφ". *)
+   (*   iDestruct (map_of_regs_2 with "HPC Hdst") as "[Hmap %]". *)
+   (*   iDestruct (extract_sep_if_split with "Ha") as "[Hflt Hr1a]". *)
+   (*   iAssert (⌜if (a =? pc_a)%a then PermFlows p pc_p' else PermFlows p p'⌝)%I with "[Hflt]" as %Hfl'. *)
+   (*   { iRevert "Hflt". destruct (a =? pc_a)%a; auto. } *)
+   (*   iDestruct (memMap_resource_2gen_clater with "Hi Hr1a") as (mem) "[>Hmem %]". *)
 
-    iApply (wp_store with "[$Hmap $Hmem]"); eauto; simplify_map_eq; eauto.
-    { by rewrite !dom_insert; set_solver+. }
-    { destruct (a =? pc_a)%a; by simplify_map_eq. }
-    { eapply mem_implies_allow_store_map; eauto. all: by simplify_map_eq. }
+   (*  iApply (wp_store with "[$Hmap $Hmem]"); eauto; simplify_map_eq; eauto. *)
+   (*  { by rewrite !dom_insert; set_solver+. } *)
+   (*  { destruct (a =? pc_a)%a; by simplify_map_eq. } *)
+   (*  { eapply mem_implies_allow_store_map; eauto. all: by simplify_map_eq. } *)
 
-    iNext. iIntros (regs' mem' retv) "(#Hspec & Hmem & Hmap)".
-    iDestruct "Hspec" as %Hspec.
+   (*  iNext. iIntros (regs' mem' retv) "(#Hspec & Hmem & Hmap)". *)
+   (*  iDestruct "Hspec" as %Hspec. *)
 
-    destruct Hspec as [ | * Hfail ].
-     { (* Success *)
-       iApply "Hφ".
-       destruct H5 as [Hrr2 _]. simplify_map_eq.
-       destruct (a0 =? pc_a)%a eqn:Heq; subst mem.
-       -  apply Z.eqb_eq, z_of_eq in Heq. subst a0.
-          rewrite insert_insert.
-          rewrite memMap_resource_1.
-          incrementPC_inv.
-          simplify_map_eq. rewrite insert_insert.
-          iDestruct (regs_of_map_2 with "[$Hmap]") as "[HPC Hsrc]"; eauto. iFrame.
+   (*  destruct Hspec as [ | * Hfail ]. *)
+   (*   { (* Success *) *)
+   (*     iApply "Hφ". *)
+   (*     destruct H5 as [Hrr2 _]. simplify_map_eq. *)
+   (*     destruct (a0 =? pc_a)%a eqn:Heq; subst mem. *)
+   (*     -  apply Z.eqb_eq, z_of_eq in Heq. subst a0. *)
+   (*        rewrite insert_insert. *)
+   (*        rewrite memMap_resource_1. *)
+   (*        incrementPC_inv. *)
+   (*        simplify_map_eq. rewrite insert_insert. *)
+   (*        iDestruct (regs_of_map_2 with "[$Hmap]") as "[HPC Hsrc]"; eauto. iFrame. *)
 
-       - apply Z.eqb_neq in Heq.
-         rewrite insert_commute; last congruence. rewrite insert_insert.
-         iDestruct (memMap_resource_2ne with "Hmem") as "[Ha0 Hpc_a]"; first congruence.
-         incrementPC_inv.
-         rewrite lookup_insert_ne in H6; last congruence. simplify_map_eq. rewrite insert_insert.
-         iDestruct (regs_of_map_2 with "[$Hmap]") as "[HPC Hsrc]"; eauto. iFrame.
-     }
-     { (* Failure (contradiction) *)
-       destruct Hfail; try incrementPC_inv; simplify_map_eq; eauto.
-       destruct o. all: try congruence.
-       destruct Hloc; first congruence. naive_solver.
-     }
-     Qed.
+   (*     - apply Z.eqb_neq in Heq. *)
+   (*       rewrite insert_commute; last congruence. rewrite insert_insert. *)
+   (*       iDestruct (memMap_resource_2ne with "Hmem") as "[Ha0 Hpc_a]"; first congruence. *)
+   (*       incrementPC_inv. *)
+   (*       rewrite lookup_insert_ne in H6; last congruence. simplify_map_eq. rewrite insert_insert. *)
+   (*       iDestruct (regs_of_map_2 with "[$Hmap]") as "[HPC Hsrc]"; eauto. iFrame. *)
+   (*   } *)
+   (*   { (* Failure (contradiction) *) *)
+   (*     destruct Hfail; try incrementPC_inv; simplify_map_eq; eauto. *)
+   (*     destruct o. all: try congruence. *)
+   (*     destruct Hloc; first congruence. naive_solver. *)
+   (*   } *)
+   (*   Qed. *)
 
-   Lemma wp_store_success_reg_same' E pc_p pc_g pc_b pc_e pc_a pc_a' w dst
-         p g b e pc_p' :
-     decodeInstrW w = Store dst (inr dst) →
-     PermFlows pc_p pc_p' →
-     PermFlows p pc_p' →
-     isCorrectPC (inr ((pc_p,pc_g),pc_b,pc_e,pc_a)) →
-     (pc_a + 1)%a = Some pc_a' →
-     writeAllowed p = true ∧ withinBounds ((p, g), b, e, pc_a) = true →
-     (isLocal g = false ∨ (p = RWLX ∨ p = RWL)) →
+   (* Lemma wp_store_success_reg_same' E pc_p pc_g pc_b pc_e pc_a pc_a' w dst *)
+   (*       p g b e pc_p' : *)
+   (*   decodeInstrW w = Store dst (inr dst) → *)
+   (*   PermFlows pc_p pc_p' → *)
+   (*   PermFlows p pc_p' → *)
+   (*   isCorrectPC (inr ((pc_p,pc_g),pc_b,pc_e,pc_a)) → *)
+   (*   (pc_a + 1)%a = Some pc_a' → *)
+   (*   writeAllowed p = true ∧ withinBounds ((p, g), b, e, pc_a) = true → *)
+   (*   (isLocal g = false ∨ (p = RWLX ∨ p = RWL)) → *)
 
-     {{{ ▷ PC ↦ᵣ inr ((pc_p,pc_g),pc_b,pc_e,pc_a)
-           ∗ ▷ pc_a ↦ₐ[pc_p'] w
-           ∗ ▷ dst ↦ᵣ inr ((p,g),b,e,pc_a) }}}
-       Instr Executable @ E
-       {{{ RET NextIV;
-           PC ↦ᵣ inr ((pc_p,pc_g),pc_b,pc_e,pc_a')
-              ∗ pc_a ↦ₐ[pc_p'] inr (p, g, b, e, pc_a)
-              ∗ dst ↦ᵣ inr ((p,g),b,e,pc_a) }}}.
-   Proof.
-     iIntros (Hinstr Hfl Hfl' Hvpc Hpca' [Hwa Hwb] Hloc φ)
-            "(>HPC & >Hi & >Hdst) Hφ".
-     iDestruct (map_of_regs_2 with "HPC Hdst") as "[Hmap %]".
-     iDestruct (memMap_resource_1 with "Hi") as "Hmem".
+   (*   {{{ ▷ PC ↦ᵣ inr ((pc_p,pc_g),pc_b,pc_e,pc_a) *)
+   (*         ∗ ▷ pc_a ↦ₐ[pc_p'] w *)
+   (*         ∗ ▷ dst ↦ᵣ inr ((p,g),b,e,pc_a) }}} *)
+   (*     Instr Executable @ E *)
+   (*     {{{ RET NextIV; *)
+   (*         PC ↦ᵣ inr ((pc_p,pc_g),pc_b,pc_e,pc_a') *)
+   (*            ∗ pc_a ↦ₐ[pc_p'] inr (p, g, b, e, pc_a) *)
+   (*            ∗ dst ↦ᵣ inr ((p,g),b,e,pc_a) }}}. *)
+   (* Proof. *)
+   (*   iIntros (Hinstr Hfl Hfl' Hvpc Hpca' [Hwa Hwb] Hloc φ) *)
+   (*          "(>HPC & >Hi & >Hdst) Hφ". *)
+   (*   iDestruct (map_of_regs_2 with "HPC Hdst") as "[Hmap %]". *)
+   (*   iDestruct (memMap_resource_1 with "Hi") as "Hmem". *)
 
-    iApply (wp_store _ pc_p with "[$Hmap $Hmem]"); eauto; simplify_map_eq; eauto.
-    { by rewrite !dom_insert; set_solver+. }
-    { eapply mem_eq_implies_allow_store_map; eauto.
-      all: by simplify_map_eq. }
-    iNext. iIntros (regs' mem' retv) "(#Hspec & Hmem & Hmap)".
-    iDestruct "Hspec" as %Hspec.
+   (*  iApply (wp_store _ pc_p with "[$Hmap $Hmem]"); eauto; simplify_map_eq; eauto. *)
+   (*  { by rewrite !dom_insert; set_solver+. } *)
+   (*  { eapply mem_eq_implies_allow_store_map; eauto. *)
+   (*    all: by simplify_map_eq. } *)
+   (*  iNext. iIntros (regs' mem' retv) "(#Hspec & Hmem & Hmap)". *)
+   (*  iDestruct "Hspec" as %Hspec. *)
 
-    destruct Hspec as [ | * Hfail ].
-     { (* Success *)
-       iApply "Hφ".
-       destruct H4 as [Hrr2 _]. simplify_map_eq.
-       rewrite memMap_resource_1.
-       incrementPC_inv.
-       simplify_map_eq.
-       do 2 rewrite insert_insert.
-       iDestruct (regs_of_map_2 with "[$Hmap]") as "[HPC Hsrc]"; eauto. iFrame. }
-     { (* Failure (contradiction) *)
-       destruct Hfail; try incrementPC_inv; simplify_map_eq; eauto.
-       destruct o. all: try congruence.
-       destruct Hloc; first congruence. naive_solver.
-     }
-   Qed.
+   (*  destruct Hspec as [ | * Hfail ]. *)
+   (*   { (* Success *) *)
+   (*     iApply "Hφ". *)
+   (*     destruct H4 as [Hrr2 _]. simplify_map_eq. *)
+   (*     rewrite memMap_resource_1. *)
+   (*     incrementPC_inv. *)
+   (*     simplify_map_eq. *)
+   (*     do 2 rewrite insert_insert. *)
+   (*     iDestruct (regs_of_map_2 with "[$Hmap]") as "[HPC Hsrc]"; eauto. iFrame. } *)
+   (*   { (* Failure (contradiction) *) *)
+   (*     destruct Hfail; try incrementPC_inv; simplify_map_eq; eauto. *)
+   (*     destruct o. all: try congruence. *)
+   (*     destruct Hloc; first congruence. naive_solver. *)
+   (*   } *)
+   (* Qed. *)
 
-   Lemma wp_store_success_reg_same_a E pc_p pc_g pc_b pc_e pc_a pc_a' w dst src
-         p g b e pc_p' w'' :
-      decodeInstrW w = Store dst (inr src) →
-      PermFlows pc_p pc_p' →
-      PermFlows p pc_p' →
-     isCorrectPC (inr ((pc_p,pc_g),pc_b,pc_e,pc_a)) →
-     (pc_a + 1)%a = Some pc_a' →
-     writeAllowed p = true ∧ withinBounds ((p, g), b, e, pc_a) = true →
-     (isLocalWord w'' = false ∨ (p = RWLX ∨ p = RWL)) →
+   (* Lemma wp_store_success_reg_same_a E pc_p pc_g pc_b pc_e pc_a pc_a' w dst src *)
+   (*       p g b e pc_p' w'' : *)
+   (*    decodeInstrW w = Store dst (inr src) → *)
+   (*    PermFlows pc_p pc_p' → *)
+   (*    PermFlows p pc_p' → *)
+   (*   isCorrectPC (inr ((pc_p,pc_g),pc_b,pc_e,pc_a)) → *)
+   (*   (pc_a + 1)%a = Some pc_a' → *)
+   (*   writeAllowed p = true ∧ withinBounds ((p, g), b, e, pc_a) = true → *)
+   (*   (isLocalWord w'' = false ∨ (p = RWLX ∨ p = RWL)) → *)
 
-     {{{ ▷ PC ↦ᵣ inr ((pc_p,pc_g),pc_b,pc_e,pc_a)
-           ∗ ▷ pc_a ↦ₐ[pc_p'] w
-           ∗ ▷ src ↦ᵣ w''
-           ∗ ▷ dst ↦ᵣ inr ((p,g),b,e,pc_a) }}}
-       Instr Executable @ E
-       {{{ RET NextIV;
-           PC ↦ᵣ inr ((pc_p,pc_g),pc_b,pc_e,pc_a')
-              ∗ pc_a ↦ₐ[pc_p'] w''
-              ∗ src ↦ᵣ w''
-              ∗ dst ↦ᵣ inr ((p,g),b,e,pc_a)}}}.
-   Proof.
-     iIntros (Hinstr Hfl Hfl' Hvpc Hpca' [Hwa Hwb] Hloc φ)
-             "(>HPC & >Hi & >Hsrc & >Hdst) Hφ".
-     iDestruct (map_of_regs_3 with "HPC Hsrc Hdst") as "[Hmap (%&%&%)]".
-     iDestruct (memMap_resource_1 with "Hi") as "Hmem".
+   (*   {{{ ▷ PC ↦ᵣ inr ((pc_p,pc_g),pc_b,pc_e,pc_a) *)
+   (*         ∗ ▷ pc_a ↦ₐ[pc_p'] w *)
+   (*         ∗ ▷ src ↦ᵣ w'' *)
+   (*         ∗ ▷ dst ↦ᵣ inr ((p,g),b,e,pc_a) }}} *)
+   (*     Instr Executable @ E *)
+   (*     {{{ RET NextIV; *)
+   (*         PC ↦ᵣ inr ((pc_p,pc_g),pc_b,pc_e,pc_a') *)
+   (*            ∗ pc_a ↦ₐ[pc_p'] w'' *)
+   (*            ∗ src ↦ᵣ w'' *)
+   (*            ∗ dst ↦ᵣ inr ((p,g),b,e,pc_a)}}}. *)
+   (* Proof. *)
+   (*   iIntros (Hinstr Hfl Hfl' Hvpc Hpca' [Hwa Hwb] Hloc φ) *)
+   (*           "(>HPC & >Hi & >Hsrc & >Hdst) Hφ". *)
+   (*   iDestruct (map_of_regs_3 with "HPC Hsrc Hdst") as "[Hmap (%&%&%)]". *)
+   (*   iDestruct (memMap_resource_1 with "Hi") as "Hmem". *)
 
-    iApply (wp_store _ pc_p with "[$Hmap $Hmem]"); eauto; simplify_map_eq; eauto.
-    { by rewrite !dom_insert; set_solver+. }
-    { eapply mem_eq_implies_allow_store_map; eauto.
-      all: by simplify_map_eq. }
-    iNext. iIntros (regs' mem' retv) "(#Hspec & Hmem & Hmap)".
-    iDestruct "Hspec" as %Hspec.
+   (*  iApply (wp_store _ pc_p with "[$Hmap $Hmem]"); eauto; simplify_map_eq; eauto. *)
+   (*  { by rewrite !dom_insert; set_solver+. } *)
+   (*  { eapply mem_eq_implies_allow_store_map; eauto. *)
+   (*    all: by simplify_map_eq. } *)
+   (*  iNext. iIntros (regs' mem' retv) "(#Hspec & Hmem & Hmap)". *)
+   (*  iDestruct "Hspec" as %Hspec. *)
 
-    destruct Hspec as [ | * Hfail ].
-     { (* Success *)
-       iApply "Hφ".
-       destruct H6 as [Hrr2 _]. simplify_map_eq.
-       rewrite memMap_resource_1.
-       incrementPC_inv.
-       simplify_map_eq.
-       do 2 rewrite insert_insert.
-       iDestruct (regs_of_map_3 with "[$Hmap]") as "[HPC [Hsrc Hdst] ]"; eauto. iFrame. }
-     { (* Failure (contradiction) *)
-       destruct Hfail; try incrementPC_inv; simplify_map_eq; eauto.
-       destruct o. all: try congruence.
-       destruct Hloc; first congruence. naive_solver.
-     }
-   Qed.
+   (*  destruct Hspec as [ | * Hfail ]. *)
+   (*   { (* Success *) *)
+   (*     iApply "Hφ". *)
+   (*     destruct H6 as [Hrr2 _]. simplify_map_eq. *)
+   (*     rewrite memMap_resource_1. *)
+   (*     incrementPC_inv. *)
+   (*     simplify_map_eq. *)
+   (*     do 2 rewrite insert_insert. *)
+   (*     iDestruct (regs_of_map_3 with "[$Hmap]") as "[HPC [Hsrc Hdst] ]"; eauto. iFrame. } *)
+   (*   { (* Failure (contradiction) *) *)
+   (*     destruct Hfail; try incrementPC_inv; simplify_map_eq; eauto. *)
+   (*     destruct o. all: try congruence. *)
+   (*     destruct Hloc; first congruence. naive_solver. *)
+   (*   } *)
+   (* Qed. *)
 
-  Lemma wp_store_success_local_reg E pc_p pc_g pc_b pc_e pc_a pc_a' w dst src w'
-         p g b e a p' g' b' e' a' pc_p' p'' :
-    decodeInstrW w = Store dst (inr src) →
-    PermFlows pc_p pc_p' →
-    PermFlows p p'' →
-     isCorrectPC (inr ((pc_p,pc_g),pc_b,pc_e,pc_a)) →
-     (pc_a + 1)%a = Some pc_a' →
-     writeAllowed p = true ∧ withinBounds ((p, g), b, e, a) = true →
-     isLocal g' = true ∧ (p = RWLX ∨ p = RWL) →
+  (* Lemma wp_store_success_local_reg E pc_p pc_g pc_b pc_e pc_a pc_a' w dst src w' *)
+  (*        p g b e a p' g' b' e' a' pc_p' p'' : *)
+  (*   decodeInstrW w = Store dst (inr src) → *)
+  (*   PermFlows pc_p pc_p' → *)
+  (*   PermFlows p p'' → *)
+  (*    isCorrectPC (inr ((pc_p,pc_g),pc_b,pc_e,pc_a)) → *)
+  (*    (pc_a + 1)%a = Some pc_a' → *)
+  (*    writeAllowed p = true ∧ withinBounds ((p, g), b, e, a) = true → *)
+  (*    isLocal g' = true ∧ (p = RWLX ∨ p = RWL) → *)
 
-     {{{ ▷ PC ↦ᵣ inr ((pc_p,pc_g),pc_b,pc_e,pc_a)
-           ∗ ▷ pc_a ↦ₐ[pc_p'] w
-           ∗ ▷ src ↦ᵣ inr ((p',g'),b',e',a')
-           ∗ ▷ dst ↦ᵣ inr ((p,g),b,e,a)
-           ∗ ▷ a ↦ₐ[p''] w' }}}
-       Instr Executable @ E
-       {{{ RET NextIV;
-           PC ↦ᵣ inr ((pc_p,pc_g),pc_b,pc_e,pc_a')
-              ∗ pc_a ↦ₐ[pc_p'] w
-              ∗ src ↦ᵣ inr ((p',g'),b',e',a')
-              ∗ dst ↦ᵣ inr ((p,g),b,e,a)
-              ∗ a ↦ₐ[p''] inr ((p',g'),b',e',a') }}}.
-  Proof.
-    iIntros (Hinstr Hfl Hfl' Hvpc Hpca' [Hwa Hwb] Hloc φ)
-             "(>HPC & >Hi & >Hsrc & >Hdst & >Hsrca) Hφ".
-    iDestruct (map_of_regs_3 with "HPC Hsrc Hdst") as "[Hmap (%&%&%)]".
-    pose proof (writeAllowed_nonO _ _ Hfl' Hwa) as Hp''.
-    pose proof (correctPC_nonO _ _ _ _ _ _ Hfl Hvpc) as Hpc_p'.
-    iDestruct (memMap_resource_2ne_apply with "Hi Hsrca") as "[Hmem %]"; auto.
+  (*    {{{ ▷ PC ↦ᵣ inr ((pc_p,pc_g),pc_b,pc_e,pc_a) *)
+  (*          ∗ ▷ pc_a ↦ₐ[pc_p'] w *)
+  (*          ∗ ▷ src ↦ᵣ inr ((p',g'),b',e',a') *)
+  (*          ∗ ▷ dst ↦ᵣ inr ((p,g),b,e,a) *)
+  (*          ∗ ▷ a ↦ₐ[p''] w' }}} *)
+  (*      Instr Executable @ E *)
+  (*      {{{ RET NextIV; *)
+  (*          PC ↦ᵣ inr ((pc_p,pc_g),pc_b,pc_e,pc_a') *)
+  (*             ∗ pc_a ↦ₐ[pc_p'] w *)
+  (*             ∗ src ↦ᵣ inr ((p',g'),b',e',a') *)
+  (*             ∗ dst ↦ᵣ inr ((p,g),b,e,a) *)
+  (*             ∗ a ↦ₐ[p''] inr ((p',g'),b',e',a') }}}. *)
+  (* Proof. *)
+  (*   iIntros (Hinstr Hfl Hfl' Hvpc Hpca' [Hwa Hwb] Hloc φ) *)
+  (*            "(>HPC & >Hi & >Hsrc & >Hdst & >Hsrca) Hφ". *)
+  (*   iDestruct (map_of_regs_3 with "HPC Hsrc Hdst") as "[Hmap (%&%&%)]". *)
+  (*   pose proof (writeAllowed_nonO _ _ Hfl' Hwa) as Hp''. *)
+  (*   pose proof (correctPC_nonO _ _ _ _ _ _ Hfl Hvpc) as Hpc_p'. *)
+  (*   iDestruct (memMap_resource_2ne_apply with "Hi Hsrca") as "[Hmem %]"; auto. *)
 
-    iApply (wp_store _ pc_p with "[$Hmap $Hmem]"); eauto; simplify_map_eq; eauto.
-    { by rewrite !dom_insert; set_solver+. }
-    { eapply mem_neq_implies_allow_store_map with (a := a) (p' := p''); eauto.
-      all: by simplify_map_eq. }
-    iNext. iIntros (regs' mem' retv) "(#Hspec & Hmem & Hmap)".
-    iDestruct "Hspec" as %Hspec.
+  (*   iApply (wp_store _ pc_p with "[$Hmap $Hmem]"); eauto; simplify_map_eq; eauto. *)
+  (*   { by rewrite !dom_insert; set_solver+. } *)
+  (*   { eapply mem_neq_implies_allow_store_map with (a := a) (p' := p''); eauto. *)
+  (*     all: by simplify_map_eq. } *)
+  (*   iNext. iIntros (regs' mem' retv) "(#Hspec & Hmem & Hmap)". *)
+  (*   iDestruct "Hspec" as %Hspec. *)
 
-    destruct Hspec as [ | * Hfail ].
-     { (* Success *)
-       iApply "Hφ".
-       destruct H7 as [Hrr2 _]. simplify_map_eq.
-       rewrite insert_commute // insert_insert.
-       iDestruct (memMap_resource_2ne with "Hmem") as "[Hpc_a Ha]";auto.
-       incrementPC_inv.
-       simplify_map_eq.
-       rewrite insert_insert.
-       iDestruct (regs_of_map_3 with "[$Hmap]") as "[HPC [Hsrc Hdst] ]"; eauto. iFrame. }
-     { (* Failure (contradiction) *)
-       destruct Hfail; try incrementPC_inv; simplify_map_eq; eauto.
-       destruct o. all: try congruence.
-       destruct Hloc as [_ Hpwl]. naive_solver.
-     }
-  Qed.
+  (*   destruct Hspec as [ | * Hfail ]. *)
+  (*    { (* Success *) *)
+  (*      iApply "Hφ". *)
+  (*      destruct H7 as [Hrr2 _]. simplify_map_eq. *)
+  (*      rewrite insert_commute // insert_insert. *)
+  (*      iDestruct (memMap_resource_2ne with "Hmem") as "[Hpc_a Ha]";auto. *)
+  (*      incrementPC_inv. *)
+  (*      simplify_map_eq. *)
+  (*      rewrite insert_insert. *)
+  (*      iDestruct (regs_of_map_3 with "[$Hmap]") as "[HPC [Hsrc Hdst] ]"; eauto. iFrame. } *)
+  (*    { (* Failure (contradiction) *) *)
+  (*      destruct Hfail; try incrementPC_inv; simplify_map_eq; eauto. *)
+  (*      destruct o. all: try congruence. *)
+  (*      destruct Hloc as [_ Hpwl]. naive_solver. *)
+  (*    } *)
+  (* Qed. *)
 
-   Lemma wp_store_success_z_reg E pc_p pc_g pc_b pc_e pc_a pc_a' w dst src w'
-         p g b e a z pc_p' p' :
-     decodeInstrW w = Store dst (inr src) →
-     PermFlows pc_p pc_p' →
-     PermFlows p p' →
-     isCorrectPC (inr ((pc_p,pc_g),pc_b,pc_e,pc_a)) →
-     (pc_a + 1)%a = Some pc_a' →
-     writeAllowed p = true ∧ withinBounds ((p, g), b, e, a) = true →
+  (*  Lemma wp_store_success_z_reg E pc_p pc_g pc_b pc_e pc_a pc_a' w dst src w' *)
+  (*        p g b e a z pc_p' p' : *)
+  (*    decodeInstrW w = Store dst (inr src) → *)
+  (*    PermFlows pc_p pc_p' → *)
+  (*    PermFlows p p' → *)
+  (*    isCorrectPC (inr ((pc_p,pc_g),pc_b,pc_e,pc_a)) → *)
+  (*    (pc_a + 1)%a = Some pc_a' → *)
+  (*    writeAllowed p = true ∧ withinBounds ((p, g), b, e, a) = true → *)
 
-     {{{ ▷ PC ↦ᵣ inr ((pc_p,pc_g),pc_b,pc_e,pc_a)
-           ∗ ▷ pc_a ↦ₐ[pc_p'] w
-           ∗ ▷ src ↦ᵣ inl z
-           ∗ ▷ dst ↦ᵣ inr ((p,g),b,e,a)
-           ∗ ▷ a ↦ₐ[p'] w' }}}
-       Instr Executable @ E
-       {{{ RET NextIV;
-           PC ↦ᵣ inr ((pc_p,pc_g),pc_b,pc_e,pc_a')
-              ∗ pc_a ↦ₐ[pc_p'] w
-              ∗ src ↦ᵣ inl z
-              ∗ dst ↦ᵣ inr ((p,g),b,e,a)
-              ∗ a ↦ₐ[p'] inl z }}}.
-   Proof.
-     iIntros (Hinstr Hfl Hfl' Hvpc Hpca' [Hwa Hwb] φ)
-             "(>HPC & >Hi & >Hsrc & >Hdst & >Hsrca) Hφ".
-    iDestruct (map_of_regs_3 with "HPC Hsrc Hdst") as "[Hmap (%&%&%)]".
-    pose proof (writeAllowed_nonO _ _ Hfl' Hwa) as Hp''.
-    pose proof (correctPC_nonO _ _ _ _ _ _ Hfl Hvpc) as Hpc_p'.
-    iDestruct (memMap_resource_2ne_apply with "Hi Hsrca") as "[Hmem %]"; auto.
+  (*    {{{ ▷ PC ↦ᵣ inr ((pc_p,pc_g),pc_b,pc_e,pc_a) *)
+  (*          ∗ ▷ pc_a ↦ₐ[pc_p'] w *)
+  (*          ∗ ▷ src ↦ᵣ inl z *)
+  (*          ∗ ▷ dst ↦ᵣ inr ((p,g),b,e,a) *)
+  (*          ∗ ▷ a ↦ₐ[p'] w' }}} *)
+  (*      Instr Executable @ E *)
+  (*      {{{ RET NextIV; *)
+  (*          PC ↦ᵣ inr ((pc_p,pc_g),pc_b,pc_e,pc_a') *)
+  (*             ∗ pc_a ↦ₐ[pc_p'] w *)
+  (*             ∗ src ↦ᵣ inl z *)
+  (*             ∗ dst ↦ᵣ inr ((p,g),b,e,a) *)
+  (*             ∗ a ↦ₐ[p'] inl z }}}. *)
+  (*  Proof. *)
+  (*    iIntros (Hinstr Hfl Hfl' Hvpc Hpca' [Hwa Hwb] φ) *)
+  (*            "(>HPC & >Hi & >Hsrc & >Hdst & >Hsrca) Hφ". *)
+  (*   iDestruct (map_of_regs_3 with "HPC Hsrc Hdst") as "[Hmap (%&%&%)]". *)
+  (*   pose proof (writeAllowed_nonO _ _ Hfl' Hwa) as Hp''. *)
+  (*   pose proof (correctPC_nonO _ _ _ _ _ _ Hfl Hvpc) as Hpc_p'. *)
+  (*   iDestruct (memMap_resource_2ne_apply with "Hi Hsrca") as "[Hmem %]"; auto. *)
 
-    iApply (wp_store _ pc_p with "[$Hmap $Hmem]"); eauto; simplify_map_eq; eauto.
-    { by rewrite !dom_insert; set_solver+. }
-    { eapply mem_neq_implies_allow_store_map with (a := a) (p' := p'); eauto.
-      all: by simplify_map_eq. }
-    iNext. iIntros (regs' mem' retv) "(#Hspec & Hmem & Hmap)".
-    iDestruct "Hspec" as %Hspec.
+  (*   iApply (wp_store _ pc_p with "[$Hmap $Hmem]"); eauto; simplify_map_eq; eauto. *)
+  (*   { by rewrite !dom_insert; set_solver+. } *)
+  (*   { eapply mem_neq_implies_allow_store_map with (a := a) (p' := p'); eauto. *)
+  (*     all: by simplify_map_eq. } *)
+  (*   iNext. iIntros (regs' mem' retv) "(#Hspec & Hmem & Hmap)". *)
+  (*   iDestruct "Hspec" as %Hspec. *)
 
-    destruct Hspec as [ | * Hfail ].
-     { (* Success *)
-       iApply "Hφ".
-       destruct H7 as [Hrr2 _]. simplify_map_eq.
-       rewrite insert_commute // insert_insert.
-       iDestruct (memMap_resource_2ne with "Hmem") as "[Hpc_a Ha]";auto.
-       incrementPC_inv.
-       simplify_map_eq.
-       rewrite insert_insert.
-       iDestruct (regs_of_map_3 with "[$Hmap]") as "[HPC [Hsrc Hdst] ]"; eauto. iFrame. }
-     { (* Failure (contradiction) *)
-       destruct Hfail; try incrementPC_inv; simplify_map_eq; eauto.
-       destruct o. all: congruence.
-     }
-   Qed.
+  (*   destruct Hspec as [ | * Hfail ]. *)
+  (*    { (* Success *) *)
+  (*      iApply "Hφ". *)
+  (*      destruct H7 as [Hrr2 _]. simplify_map_eq. *)
+  (*      rewrite insert_commute // insert_insert. *)
+  (*      iDestruct (memMap_resource_2ne with "Hmem") as "[Hpc_a Ha]";auto. *)
+  (*      incrementPC_inv. *)
+  (*      simplify_map_eq. *)
+  (*      rewrite insert_insert. *)
+  (*      iDestruct (regs_of_map_3 with "[$Hmap]") as "[HPC [Hsrc Hdst] ]"; eauto. iFrame. } *)
+  (*    { (* Failure (contradiction) *) *)
+  (*      destruct Hfail; try incrementPC_inv; simplify_map_eq; eauto. *)
+  (*      destruct o. all: congruence. *)
+  (*    } *)
+  (*  Qed. *)
 
     Lemma wp_store_success_reg E pc_p pc_g pc_b pc_e pc_a pc_a' w dst src w'
          p g b e a w'' pc_p' p' :
@@ -784,7 +794,8 @@ Section cap_lang_rules.
      isCorrectPC (inr ((pc_p,pc_g),pc_b,pc_e,pc_a)) →
      (pc_a + 1)%a = Some pc_a' →
      writeAllowed p = true ∧ withinBounds ((p, g), b, e, a) = true →
-     (isLocalWord w'' = false ∨ (p = RWLX ∨ p = RWL)) →
+     canStore p a w'' = true ->
+     (* (isLocalWord w'' = false ∨ (p = RWLX ∨ p = RWL)) → *)
 
      {{{ ▷ PC ↦ᵣ inr ((pc_p,pc_g),pc_b,pc_e,pc_a)
            ∗ ▷ pc_a ↦ₐ[pc_p'] w
@@ -826,7 +837,6 @@ Section cap_lang_rules.
      { (* Failure (contradiction) *)
        destruct Hfail; try incrementPC_inv; simplify_map_eq; eauto.
        destruct o. all: try congruence.
-       destruct Hloc as [Hlw | Hpwl]; first congruence. naive_solver.
      }
     Qed.
 
@@ -838,7 +848,8 @@ Section cap_lang_rules.
      isCorrectPC (inr ((pc_p,pc_g),pc_b,pc_e,pc_a)) →
      (pc_a + 1)%a = Some pc_a' →
      writeAllowed p = true ∧ withinBounds ((p, g), b, e, a) = true →
-     (isLocal g = false ∨ (p = RWLX ∨ p = RWL)) →
+     canStore p a (inr ((p,g),b,e,a)) = true ->
+     (* (isLocal g = false ∨ (p = RWLX ∨ p = RWL)) → *)
 
      {{{ ▷ PC ↦ᵣ inr ((pc_p,pc_g),pc_b,pc_e,pc_a)
            ∗ ▷ pc_a ↦ₐ[pc_p'] w
@@ -878,7 +889,6 @@ Section cap_lang_rules.
      { (* Failure (contradiction) *)
        destruct Hfail; try incrementPC_inv; simplify_map_eq; eauto.
        destruct o. all: try congruence.
-       destruct Hloc as [Hlw | Hpwl]; first congruence. naive_solver.
      }
     Qed.
 
@@ -930,6 +940,6 @@ Section cap_lang_rules.
        destruct Hfail; try incrementPC_inv; simplify_map_eq; eauto.
        destruct o. all: try congruence.
      }
-    Qed.
+   Qed.
 
  End cap_lang_rules.
