theories/rules/rules_StoreU_derived.v
@@ -3,17 +3,17 @@ From iris.base_logic Require Export invariants gen_heap.
 From iris.program_logic Require Export weakestpre ectx_lifting.
 From iris.proofmode Require Import tactics.
 From iris.algebra Require Import frac.
-From cap_machine.rules Require Import rules_StoreU. 
+From cap_machine.rules Require Import rules_StoreU.
 
 Section cap_lang_rules.
   Context `{memG Σ, regG Σ, MonRef: MonRefG (leibnizO _) CapR_rtc Σ}.
   Context `{MachineParameters}.
   Implicit Types P Q : iProp Σ.
   Implicit Types σ : ExecConf.
-  Implicit Types c : cap_lang.expr. 
+  Implicit Types c : cap_lang.expr.
   Implicit Types a b : Addr.
   Implicit Types r : RegName.
-  Implicit Types v : cap_lang.val. 
+  Implicit Types v : cap_lang.val.
   Implicit Types w : Word.
   Implicit Types reg : gmap RegName Word.
   Implicit Types ms : gmap Addr Word.
@@ -33,17 +33,17 @@ Section cap_lang_rules.
             then if Addr_le_dec a' a then if Addr_lt_dec a e then Some a' else None else None
             else None
         | None => None
-        end = Some a. 
+        end = Some a.
   Proof.
-    intros b e a Hwb. 
-    rewrite /= addr_add_0 /=. 
+    intros b e a Hwb.
+    rewrite /= addr_add_0 /=.
     apply withinBounds_le_addr in Hwb as [Hle Hlt].
     destruct (Addr_le_dec b a);[|contradiction].
     destruct (Addr_le_dec a a);[|solve_addr].
     destruct (Addr_lt_dec a e);[|contradiction].
-    auto. 
+    auto.
   Qed.
-  
+
   (* store and increment *)
   Lemma wp_storeU_success_0_reg E pc_p pc_g pc_b pc_e pc_a pc_a' w dst src w'
          p g b e a a' w'' pc_p' p' :
@@ -52,10 +52,10 @@ Section cap_lang_rules.
     PermFlows p p' →
     isCorrectPC (inr ((pc_p,pc_g),pc_b,pc_e,pc_a)) →
     (pc_a + 1)%a = Some pc_a' →
-    isU p  = true -> canStoreU p w'' = true ->
+    isU p  = true -> canStoreU p a w'' = true ->
     withinBounds ((p, g), b, e, a) = true ->
     (a + 1)%a = Some a' ->
-    
+
 
      {{{ ▷ PC ↦ᵣ inr ((pc_p,pc_g),pc_b,pc_e,pc_a)
            ∗ ▷ pc_a ↦ₐ[pc_p'] w
@@ -69,7 +69,7 @@ Section cap_lang_rules.
               ∗ src ↦ᵣ w''
               ∗ dst ↦ᵣ inr ((p,g),b,e,a')
               ∗ a ↦ₐ[p'] w'' }}}.
-    Proof.
+  Proof.
       iIntros (Hinstr Hfl Hfl' Hvpc Hpca' HU HstoreU Hwb Ha' φ)
              "(>HPC & >Hi & >Hsrc & >Hdst & >Hsrca) Hφ".
     iDestruct (map_of_regs_3 with "HPC Hsrc Hdst") as "[Hmap (%&%&%)]".
@@ -79,7 +79,7 @@ Section cap_lang_rules.
 
     iApply (wp_storeU _ pc_p with "[$Hmap $Hmem]"); eauto; simplify_map_eq; eauto.
     { by rewrite !dom_insert; set_solver+. }
-    { rewrite HU HstoreU. erewrite wb_implies_verify_access; eauto. 
+    { rewrite HU HstoreU. erewrite wb_implies_verify_access; eauto.
       by simplify_map_eq. }
     iNext. iIntros (regs' mem' retv) "(#Hspec & Hmem & Hmap)".
     iDestruct "Hspec" as %Hspec.
@@ -91,19 +91,19 @@ Section cap_lang_rules.
        erewrite wb_implies_verify_access in H11; eauto. simplify_eq.
        rewrite insert_commute // insert_insert.
        iDestruct (memMap_resource_2ne with "Hmem") as "[Hpc_a Ha]";auto.
-       destruct (addr_eq_dec a'0 a'0);[|contradiction]. 
+       destruct (addr_eq_dec a'0 a'0);[|contradiction].
        incrementPC_inv.
        simplify_map_eq.
        rewrite (insert_commute _ _ PC) // insert_insert.
-       rewrite (insert_commute _ _ src) // insert_insert. 
+       rewrite (insert_commute _ _ src) // insert_insert.
        iDestruct (regs_of_map_3 with "[$Hmap]") as "[HPC [Hsrc Hdst] ]"; eauto. iFrame. }
      { (* Failure (contradiction) *)
        destruct Hfail; try incrementPC_inv; simplify_map_eq; eauto.
        all: try congruence.
-       erewrite wb_implies_verify_access in e6; eauto. simplify_eq. 
-       Unshelve. all:auto. 
+       erewrite wb_implies_verify_access in e6; eauto. simplify_eq.
+       Unshelve. all:auto.
      }
-    Qed.
+  Qed.
 
   (* store and increment from and to the same register *)
   Lemma wp_storeU_success_0_reg_same E pc_p pc_g pc_b pc_e pc_a pc_a' w dst w'
@@ -113,7 +113,7 @@ Section cap_lang_rules.
     PermFlows p p' →
     isCorrectPC (inr ((pc_p,pc_g),pc_b,pc_e,pc_a)) →
     (pc_a + 1)%a = Some pc_a' →
-    isU p  = true -> canStoreU p (inr (p, g, b, e, a)) = true ->
+    isU p  = true -> canStoreU p a (inr (p, g, b, e, a)) = true ->
     withinBounds ((p, g), b, e, a) = true ->
     (a + 1)%a = Some a' ->
 
@@ -128,8 +128,8 @@ Section cap_lang_rules.
               ∗ pc_a ↦ₐ[pc_p'] w
               ∗ dst ↦ᵣ inr ((p,g),b,e,a')
               ∗ a ↦ₐ[p'] inr ((p,g),b,e,a)}}}.
-    Proof.
-      iIntros (Hinstr Hfl Hfl' Hvpc Hpca' HU HstoreU Hwb Ha' φ)
+  Proof.
+    iIntros (Hinstr Hfl Hfl' Hvpc Hpca' HU HstoreU Hwb Ha' φ)
              "(>HPC & >Hi & >Hdst & >Hsrca) Hφ".
     iDestruct (map_of_regs_2 with "HPC Hdst") as "[Hmap %]".
     pose proof (isU_nonO _ _ Hfl' HU) as Hp''.
@@ -162,19 +162,19 @@ Section cap_lang_rules.
        erewrite wb_implies_verify_access in e6; eauto. simplify_eq.
        Unshelve. all:auto.
      }
-    Qed.
+  Qed.
 
-    Lemma wp_storeU_success_0_z E pc_p pc_g pc_b pc_e pc_a pc_a' w dst z w'
+  Lemma wp_storeU_success_0_z E pc_p pc_g pc_b pc_e pc_a pc_a' w dst z w'
          p g b e a a' pc_p' p' :
     decodeInstrW w = StoreU dst (inl 0%Z) (inl z) →
     PermFlows pc_p pc_p' →
     PermFlows p p' →
     isCorrectPC (inr ((pc_p,pc_g),pc_b,pc_e,pc_a)) →
     (pc_a + 1)%a = Some pc_a' →
-    isU p  = true -> 
+    isU p  = true ->
     withinBounds ((p, g), b, e, a) = true ->
     (a + 1)%a = Some a' ->
-    
+
 
      {{{ ▷ PC ↦ᵣ inr ((pc_p,pc_g),pc_b,pc_e,pc_a)
            ∗ ▷ pc_a ↦ₐ[pc_p'] w
@@ -186,8 +186,8 @@ Section cap_lang_rules.
               ∗ pc_a ↦ₐ[pc_p'] w
               ∗ dst ↦ᵣ inr ((p,g),b,e,a')
               ∗ a ↦ₐ[p'] (inl z) }}}.
-    Proof.
-      iIntros (Hinstr Hfl Hfl' Hvpc Hpca' HU Hwb Ha' φ)
+  Proof.
+    iIntros (Hinstr Hfl Hfl' Hvpc Hpca' HU Hwb Ha' φ)
              "(>HPC & >Hi & >Hdst & >Hsrca) Hφ".
     iDestruct (map_of_regs_2 with "HPC Hdst") as "[Hmap %]".
     pose proof (isU_nonO _ _ Hfl' HU) as Hp''.
@@ -196,7 +196,7 @@ Section cap_lang_rules.
 
     iApply (wp_storeU _ pc_p with "[$Hmap $Hmem]"); eauto; simplify_map_eq; eauto.
     { by rewrite !dom_insert; set_solver+. }
-    { rewrite HU. erewrite wb_implies_verify_access; eauto. 
+    { rewrite HU. erewrite wb_implies_verify_access; eauto.
       by simplify_map_eq. }
     iNext. iIntros (regs' mem' retv) "(#Hspec & Hmem & Hmap)".
     iDestruct "Hspec" as %Hspec.
@@ -208,18 +208,17 @@ Section cap_lang_rules.
        erewrite wb_implies_verify_access in H9; eauto. simplify_eq.
        rewrite insert_commute // insert_insert.
        iDestruct (memMap_resource_2ne with "Hmem") as "[Hpc_a Ha]";auto.
-       destruct (addr_eq_dec a'0 a'0);[|contradiction]. 
+       destruct (addr_eq_dec a'0 a'0);[|contradiction].
        incrementPC_inv.
        simplify_map_eq.
-       rewrite (insert_commute _ _ PC) // insert_insert. rewrite insert_insert. 
+       rewrite (insert_commute _ _ PC) // insert_insert. rewrite insert_insert.
        iDestruct (regs_of_map_2 with "[$Hmap]") as "[HPC Hdst]"; eauto. iFrame. }
      { (* Failure (contradiction) *)
        destruct Hfail; try incrementPC_inv; simplify_map_eq; eauto.
        all: try congruence.
-       erewrite wb_implies_verify_access in e6; eauto. simplify_eq. 
-       Unshelve. all:auto. 
+       erewrite wb_implies_verify_access in e6; eauto. simplify_eq.
+       Unshelve. all:auto.
      }
-    Qed.
+  Qed.
 
-
-End cap_lang_rules. 
+End cap_lang_rules.
